Increment-only_counter/App.fst
@@ -16,8 +16,11 @@ let init_st = 0
 // (the only operation is increment, so unit is fine)
 type op_t = unit
 
+// concrete do pre-condition
+let concrete_do_pre _ _ = true
+
 // apply an operation to a state
-let do (s:concrete_st) (_:log_entry) : concrete_st = s + 1
+let do (s:concrete_st) (op:log_entry{concrete_do_pre s op}) : concrete_st = s + 1
 
 ////////////////////////////////////////////////////////////////
 //// Sequential implementation //////
@@ -47,8 +50,10 @@ let do_eq (st_s:concrete_st_s) (st:concrete_st) (op:log_entry)
 ////////////////////////////////////////////////////////////////
 
 let rec lem_foldl (s:concrete_st) (l:log)
-  : Lemma (ensures (seq_foldl s l = s + length l) /\
-                   (length l > 0 ==> (seq_foldl s l = seq_foldl s (fst (un_snoc l)) + 1)))
+  : Lemma (requires foldl_prop s l)
+          (ensures (seq_foldl s l = s + length l) /\
+                   (length l > 0 ==> (foldl_prop s (fst (un_snoc l)) /\
+                                     seq_foldl s l = seq_foldl s (fst (un_snoc l)) + 1)))
           (decreases length l)
   = match length l with
     |0 -> ()
@@ -63,8 +68,8 @@ let concrete_merge_pre lca a b : prop
   = a >= lca /\ b >= lca
 
 // concrete merge operation
-let concrete_merge (lca:concrete_st) (cst1:concrete_st) (cst2:concrete_st{concrete_merge_pre lca cst1 cst2}) 
-  : concrete_st = cst1 + cst2 - lca
+let concrete_merge (lca:concrete_st) (s1:concrete_st) (s2:concrete_st{concrete_merge_pre lca s1 s2}) 
+  : concrete_st = s1 + s2 - lca
 
 #set-options "--z3rlimit 50"
 let merge_prop (lca s1 s2:st)
@@ -98,7 +103,8 @@ let linearizable_s1_0 (lca s1 s2:st)
       (requires concrete_merge_pre (v_of lca) (v_of s1) (v_of s2) /\
                 is_prefix (ops_of lca) (ops_of s1) /\
                 is_prefix (ops_of lca) (ops_of s2) /\
-                ops_of s1 = ops_of lca)
+                ops_of s1 = ops_of lca /\
+                foldl_prop (v_of lca) (diff (ops_of s2) (ops_of lca)))
       (ensures concrete_merge (v_of lca) (v_of s1) (v_of s2) == 
                seq_foldl (v_of lca) (diff (ops_of s2) (ops_of lca))) =
   lem_foldl (v_of lca) (diff (ops_of s2) (ops_of lca));
@@ -110,7 +116,8 @@ let linearizable_s2_0 (lca s1 s2:st)
       (requires concrete_merge_pre (v_of lca) (v_of s1) (v_of s2) /\
                 is_prefix (ops_of lca) (ops_of s1) /\
                 is_prefix (ops_of lca) (ops_of s2) /\
-                ops_of s2 = ops_of lca)
+                ops_of s2 = ops_of lca /\
+                foldl_prop (v_of lca) (diff (ops_of s1) (ops_of lca)))
       (ensures concrete_merge (v_of lca) (v_of s1) (v_of s2) == 
                seq_foldl (v_of lca) (diff (ops_of s1) (ops_of lca))) =
   lem_foldl (v_of lca) (diff (ops_of s1) (ops_of lca));
@@ -126,12 +133,16 @@ let linearizable_s1_gt0 (lca s1 s2:st)
   : Lemma 
       (requires is_prefix (ops_of lca) (ops_of s1) /\
                 is_prefix (ops_of lca) (ops_of s2) /\
-                Seq.length (ops_of s1) > Seq.length (ops_of lca) /\
+                Seq.length (ops_of s1) > Seq.length (ops_of lca) /\ 
                 is_prefix (ops_of lca) (ops_of (inverse_st s1)) /\
                 concrete_merge_pre (v_of lca) (v_of s1) (v_of s2) /\
                 concrete_merge_pre (v_of lca) (v_of (inverse_st s1)) (v_of s2))
-      (ensures concrete_merge (v_of lca) (v_of s1) (v_of s2) ==
-               do (concrete_merge (v_of lca) (v_of (inverse_st s1)) (v_of s2)) (Seq.last (ops_of s1))) =
+      (ensures (let _, last1 = un_snoc (ops_of s1) in
+                concrete_do_pre (concrete_merge (v_of lca) (v_of (inverse_st s1)) (v_of s2)) last1 /\
+                concrete_merge (v_of lca) (v_of s1) (v_of s2) ==
+                do (concrete_merge (v_of lca) (v_of (inverse_st s1)) (v_of s2)) last1)) = 
+  let _,last1 = un_snoc (ops_of s1) in
+  assert (concrete_do_pre (concrete_merge (v_of lca) (v_of (inverse_st s1)) (v_of s2)) last1);
   lem_add (v_of lca) (v_of s1) (v_of s2)
 
 let linearizable_s2_gt0 (lca s1 s2:st)
@@ -142,6 +153,10 @@ let linearizable_s2_gt0 (lca s1 s2:st)
                 is_prefix (ops_of lca) (ops_of (inverse_st s2)) /\
                 concrete_merge_pre (v_of lca) (v_of s1) (v_of s2) /\
                 concrete_merge_pre (v_of lca) (v_of s1) (v_of (inverse_st s2)))
-      (ensures concrete_merge (v_of lca) (v_of s1) (v_of s2) ==
-               do (concrete_merge (v_of lca) (v_of s1) (v_of (inverse_st s2))) (Seq.last (ops_of s2))) =
- lem_add (v_of lca) (v_of s1) (v_of s2)
+      (ensures (let _, last2 = un_snoc (ops_of s2) in
+                concrete_do_pre (concrete_merge (v_of lca) (v_of s1) (v_of (inverse_st s2))) last2 /\
+                concrete_merge (v_of lca) (v_of s1) (v_of s2) ==
+                do (concrete_merge (v_of lca) (v_of s1) (v_of (inverse_st s2))) last2)) =
+  let _,last2 = un_snoc (ops_of s2) in
+  assert (concrete_do_pre (concrete_merge (v_of lca) (v_of s1) (v_of (inverse_st s2))) last2);
+  lem_add (v_of lca) (v_of s1) (v_of s2)
