PN_counter/App.fst
@@ -17,8 +17,11 @@ type op_t:eqtype =
   |Inc
   |Dec
 
+// concrete do pre-condition
+let concrete_do_pre _ _ = true
+
 // apply an operation to a state
-let do (s:concrete_st) (op:log_entry) : concrete_st = 
+let do (s:concrete_st) (op:log_entry{concrete_do_pre s op}) : concrete_st = 
   match snd op with
   |Inc -> s + 1
   |Dec -> s - 1
@@ -68,9 +71,12 @@ let rec count_dec (l:log) : Tot nat (decreases length l) =
        |_ -> count_dec (tail l)
 
 let rec lem_foldl (s:concrete_st) (l:log)
-  : Lemma (ensures (seq_foldl s l = s + count_inc l - count_dec l) /\
-                   (length l > 0 /\ snd (Seq.last l) = Inc  ==> (seq_foldl s l = seq_foldl s (fst (Seq.un_snoc l)) + 1)) /\
-                   (length l > 0 /\ snd (Seq.last l) = Dec  ==> (seq_foldl s l = seq_foldl s (fst (Seq.un_snoc l)) - 1)))
+  : Lemma (requires foldl_prop s l)
+          (ensures (seq_foldl s l = s + count_inc l - count_dec l) /\
+                   (length l > 0 /\ snd (Seq.last l) = Inc ==> 
+                           (foldl_prop s (fst (Seq.un_snoc l)) /\ seq_foldl s l = seq_foldl s (fst (Seq.un_snoc l)) + 1)) /\
+                   (length l > 0 /\ snd (Seq.last l) = Dec ==>
+                           (foldl_prop s (fst (Seq.un_snoc l)) /\ seq_foldl s l = seq_foldl s (fst (Seq.un_snoc l)) - 1)))
           (decreases length l)
   = match length l with
     |0 -> ()
@@ -84,8 +90,8 @@ let resolve_conflict (x y:log_entry) : log =
 let concrete_merge_pre lca a b : prop = true
 
 // concrete merge operation
-let concrete_merge (lca:concrete_st) (cst1:concrete_st) (cst2:concrete_st{concrete_merge_pre lca cst1 cst2}) 
-  : concrete_st = cst1 + cst2 - lca
+let concrete_merge (lca:concrete_st) (s1:concrete_st) (s2:concrete_st{concrete_merge_pre lca s1 s2}) 
+  : concrete_st = s1 + s2 - lca
 
 #push-options "--z3rlimit 50"
 let merge_prop (lca s1 s2:st)
@@ -121,7 +127,8 @@ let linearizable_s1_0 (lca s1 s2:st)
       (requires concrete_merge_pre (v_of lca) (v_of s1) (v_of s2) /\
                 is_prefix (ops_of lca) (ops_of s1) /\
                 is_prefix (ops_of lca) (ops_of s2) /\
-                ops_of s1 = ops_of lca)
+                ops_of s1 = ops_of lca /\
+                foldl_prop (v_of lca) (diff (ops_of s2) (ops_of lca)))
       (ensures concrete_merge (v_of lca) (v_of s1) (v_of s2) == 
                seq_foldl (v_of lca) (diff (ops_of s2) (ops_of lca))) =
   lem_foldl init_st (ops_of lca);
@@ -135,7 +142,8 @@ let linearizable_s2_0 (lca s1 s2:st)
       (requires concrete_merge_pre (v_of lca) (v_of s1) (v_of s2) /\
                 is_prefix (ops_of lca) (ops_of s1) /\
                 is_prefix (ops_of lca) (ops_of s2) /\
-                ops_of s2 = ops_of lca)
+                ops_of s2 = ops_of lca /\
+                foldl_prop (v_of lca) (diff (ops_of s1) (ops_of lca)))
       (ensures concrete_merge (v_of lca) (v_of s1) (v_of s2) == 
                seq_foldl (v_of lca) (diff (ops_of s1) (ops_of lca))) =
   lem_foldl init_st (ops_of lca);
@@ -159,8 +167,12 @@ let linearizable_s1_gt0 (lca s1 s2:st)
                 is_prefix (ops_of lca) (ops_of (inverse_st s1)) /\
                 concrete_merge_pre (v_of lca) (v_of s1) (v_of s2) /\
                 concrete_merge_pre (v_of lca) (v_of (inverse_st s1)) (v_of s2))
-      (ensures concrete_merge (v_of lca) (v_of s1) (v_of s2) ==
-               do (concrete_merge (v_of lca) (v_of (inverse_st s1)) (v_of s2)) (Seq.last (ops_of s1))) =
+      (ensures (let _, last1 = un_snoc (ops_of s1) in
+                concrete_do_pre (concrete_merge (v_of lca) (v_of (inverse_st s1)) (v_of s2)) last1 /\
+                concrete_merge (v_of lca) (v_of s1) (v_of s2) ==
+                do (concrete_merge (v_of lca) (v_of (inverse_st s1)) (v_of s2)) last1)) =
+  let _, last1 = un_snoc (ops_of s1) in
+  assert (concrete_do_pre (concrete_merge (v_of lca) (v_of (inverse_st s1)) (v_of s2)) last1);
   lem_add (v_of lca) (v_of s1) (v_of s2)
 
 let linearizable_s2_gt0 (lca s1 s2:st)
@@ -171,6 +183,10 @@ let linearizable_s2_gt0 (lca s1 s2:st)
                 is_prefix (ops_of lca) (ops_of (inverse_st s2)) /\
                 concrete_merge_pre (v_of lca) (v_of s1) (v_of s2) /\
                 concrete_merge_pre (v_of lca) (v_of s1) (v_of (inverse_st s2)))
-      (ensures concrete_merge (v_of lca) (v_of s1) (v_of s2) ==
-               do (concrete_merge (v_of lca) (v_of s1) (v_of (inverse_st s2))) (Seq.last (ops_of s2))) =
+      (ensures (let _, last2 = un_snoc (ops_of s2) in
+                concrete_do_pre (concrete_merge (v_of lca) (v_of s1) (v_of (inverse_st s2))) last2 /\
+                concrete_merge (v_of lca) (v_of s1) (v_of s2) ==
+                do (concrete_merge (v_of lca) (v_of s1) (v_of (inverse_st s2))) last2)) =
+  let _, last2 = un_snoc (ops_of s2) in
+  assert (concrete_do_pre (concrete_merge (v_of lca) (v_of s1) (v_of (inverse_st s2))) last2);
   lem_add (v_of lca) (v_of s1) (v_of s2)
